cfi/refinementSC.v
@@ -658,6 +658,57 @@ Qed.
 Definition khandler := @rules.handler cfi_tag_eqType mt ops e (@Symbolic.handler mt sym_params).
 Definition uhandler := @Symbolic.handler mt sym_params.
 
+(*XXX: Move these to refinement_common*)
+Lemma get_reg_no_user sreg reg r v ctg t :
+  @refinement_common.refine_registers mt ops sym_params cp e sreg reg ->
+  get sreg r = None ->
+  TotalMaps.get reg r = v@ctg ->
+  rules.decode ctg = Some t ->
+  t = rules.KERNEL \/ (exists ut, t = rules.ENTRY ut).
+Proof.
+  intros REF SGET GET DEC.
+  destruct t.
+  - apply rules.encodeK in DEC.
+    rewrite <- DEC in GET.
+    apply REF in GET.
+    rewrite SGET in GET. discriminate.
+  - auto.
+  - right; eexists; reflexivity.
+Qed.
+
+Lemma get_mem_no_user smem mem addr v ctg t :
+  @refinement_common.refine_memory mt ops sym_params cp e smem mem ->
+  get smem addr = None ->
+  get mem addr = Some v@ctg ->
+  rules.decode ctg = Some t ->
+  t = rules.KERNEL \/ (exists ut, t = rules.ENTRY ut).
+Proof.
+  intros REF SGET GET DEC.
+  destruct t.
+  - apply rules.encodeK in DEC.
+    rewrite <- DEC in GET.
+    apply REF in GET.
+    rewrite SGET in GET. discriminate.
+  - auto.
+  - right; eexists; reflexivity.
+Qed.
+
+Lemma in_user_ctpc cst :
+  @refinement_common.in_user mt ops sym_params cp e cst = true ->
+  exists ut, 
+    rules.decode (common.tag (Concrete.pc cst)) = Some (rules.USER ut).
+Proof.
+  intros USER.
+  unfold refinement_common.in_user in USER.
+  unfold rules.word_lift in USER.
+  destruct (rules.decode (common.tag (Concrete.pc cst))) eqn:DEC.
+  - destruct t.
+    + eexists; reflexivity.
+    + simpl in USER. discriminate.
+    + simpl in USER. discriminate.
+  - discriminate.
+Qed.
+
 (*Case 1: umvec = Some & cmvec = Some*)
 
 Lemma umvec_implies_cmvec sst cst smvec :
@@ -767,60 +818,85 @@ Lemma unique_cmvec sst cst umvec cmvec :
   build_cmvec mt cst = Some cmvec ->
   rules.encode_mvec (rules.mvec_of_umvec umvec) = cmvec.
 Proof.
-  Admitted.
+  intros REF UMVEC CMVEC.
+  destruct sst as [smem sreg [spc tpc] int].
+  destruct cst as [mem reg cache [pc ctpc] epc].
+  destruct REF as [PC [TPC [REFM [REFR [CACHE [MVEC [WF KI]]]]]]].
+  destruct (rules.decode ctpc) eqn:CTPC; try contradiction.
+  destruct t; try contradiction.
+  apply rules.encodeK in CTPC.
+  subst.
+  unfold build_mvec in UMVEC.
+  destruct (get smem pc) eqn:SGET.
+  - destruct a as [v tg]. simpl in UMVEC.
+    destruct (decode_instr v) eqn:DEC.
+    + destruct i eqn:OP;
+      unfold bind in UMVEC;
+      repeat match goal with
+               | [H: match ?Expr with _ => _ end = _|- _] => 
+                 remember (Expr) as hexpr; destruct hexpr
+             end;
+      repeat match goal with
+               | [H: Some ?A = get _ _ |- _] => destruct A; symmetry in H
+             end;
+      repeat match goal with
+               | [H : get sreg _ = Some _ |- _] => 
+                 apply REFR in H
+               | [H : get smem _ = Some _ |- _] => 
+                 apply REFM in H
+             end;
+      unfold build_cmvec, bind in CMVEC;
+      repeat match goal with
+               | [H: match ?Expr with _ => _ end = _, H': ?Expr = _ |- _] => 
+                 rewrite H' in H; simpl in H'
+             end;
+      inv CMVEC;
+      inv UMVEC;
+      repeat match goal with 
+               | [H: TotalMaps.get _ _ = _ |- _] => rewrite H
+             end;
+      unfold rules.mvec_of_umvec; simpl;
+      unfold rules.encode_mvec; simpl;
+      try reflexivity.
+      (*handling automation fails*)
+      * rewrite Heqhexpr in H0.
+        simpl in H0.
+        simpl in Heqhexpr0.
+        rewrite Heqhexpr0 in H0.
+        inv H0. rewrite Heqhexpr1.
+        reflexivity.
+      * rewrite Heqhexpr in H0.
+        simpl in H0. simpl in Heqhexpr1. rewrite Heqhexpr1 in H0.
+        inv H0.
+        rewrite Heqhexpr0.
+        reflexivity.
+    + discriminate.
+  - destruct (Symbolic.get_syscall stable pc) eqn:GETCALL.
+    { (*syscall case*)
+      inv UMVEC.
+      unfold rules.mvec_of_umvec. simpl.
+      unfold rules.encode_mvec. simpl.
+      remember (Symbolic.entry_tag s) as etag eqn:ETAG. symmetry in ETAG.
+      unfold wf_entry_points in WF.
+      specialize (WF pc etag).
+      assert (ECALL : (exists sc : Symbolic.syscall mt,
+          Symbolic.get_syscall stable pc = Some sc /\
+          Symbolic.entry_tag sc = etag))
+        by (eexists; eauto).
+      apply WF in ECALL.
+      destruct (get mem pc) eqn:GET.
+      destruct a. apply andb_true_iff in ECALL.
+      destruct ECALL as [VAL TG].
+      move/eqP:VAL => VAL.
+      move/eqP:TG => TG.
+      unfold build_cmvec in CMVEC.
+      rewrite GET in CMVEC. simpl in CMVEC. rewrite VAL in CMVEC.
+      rewrite common.decodeK in CMVEC. inv CMVEC.
+      Admitted.
+   
+
 
 (*Case 2*)
-(*XXX: Move these to refinement_common*)
-Lemma get_reg_no_user sreg reg r v ctg t :
-  @refinement_common.refine_registers mt ops sym_params cp e sreg reg ->
-  get sreg r = None ->
-  TotalMaps.get reg r = v@ctg ->
-  rules.decode ctg = Some t ->
-  t = rules.KERNEL \/ (exists ut, t = rules.ENTRY ut).
-Proof.
-  intros REF SGET GET DEC.
-  destruct t.
-  - apply rules.encodeK in DEC.
-    rewrite <- DEC in GET.
-    apply REF in GET.
-    rewrite SGET in GET. discriminate.
-  - auto.
-  - right; eexists; reflexivity.
-Qed.
-
-Lemma get_mem_no_user smem mem addr v ctg t :
-  @refinement_common.refine_memory mt ops sym_params cp e smem mem ->
-  get smem addr = None ->
-  get mem addr = Some v@ctg ->
-  rules.decode ctg = Some t ->
-  t = rules.KERNEL \/ (exists ut, t = rules.ENTRY ut).
-Proof.
-  intros REF SGET GET DEC.
-  destruct t.
-  - apply rules.encodeK in DEC.
-    rewrite <- DEC in GET.
-    apply REF in GET.
-    rewrite SGET in GET. discriminate.
-  - auto.
-  - right; eexists; reflexivity.
-Qed.
-
-Lemma in_user_ctpc cst :
-  @refinement_common.in_user mt ops sym_params cp e cst = true ->
-  exists ut, 
-    rules.decode (common.tag (Concrete.pc cst)) = Some (rules.USER ut).
-Proof.
-  intros USER.
-  unfold refinement_common.in_user in USER.
-  unfold rules.word_lift in USER.
-  destruct (rules.decode (common.tag (Concrete.pc cst))) eqn:DEC.
-  - destruct t.
-    + eexists; reflexivity.
-    + simpl in USER. discriminate.
-    + simpl in USER. discriminate.
-  - discriminate.
-Qed.
-
 Lemma no_user_access_implies_halt sst cst cmvec :
   refinement_common.refine_state ki stable sst cst ->
   build_mvec stable sst = None ->
@@ -952,8 +1028,24 @@ Proof. (*Postpone proof until khandler rewrite*) Admitted.
 Lemma concrete_stuck cst :
   build_cmvec mt cst = None ->
   ~exists cst', Concrete.step _ masks cst cst'.
-Proof. Admitted.
-
+Proof. 
+  intros CMVEC (cst' & STEP).
+  destruct cst as [mem reg cache [pc tpc] epc].
+  inversion STEP; inversion ST;
+  unfold build_cmvec in CMVEC;
+  subst;
+  simpl in CMVEC;
+  repeat (match goal with 
+    | [H: ?Expr = _, H' : match ?Expr with _ => _ end = _ |- _] => 
+      rewrite H in H'
+          end);
+  try discriminate.
+  rewrite REG1 in CMVEC.
+  simpl in CMVEC. rewrite M1 in CMVEC. simpl in CMVEC. discriminate.
+  rewrite REG1 in CMVEC. simpl in CMVEC. rewrite M1 in CMVEC.
+  simpl in CMVEC. discriminate.
+Qed.
+  
 (*Move to refinement_common?*)
 (*Again rough statement, subject to change*)
 Lemma fault_steps_at_kernel ast cst cst' cmvec :
